lib/CompileFirstOrderConfRelSimplified.v
@@ -28,9 +28,9 @@ Section CompileFirstOrderConfRelSimplified.
   Variable (Hdr: Type).
   Context `{Hdr_eq_dec: EquivDec.EqDec Hdr eq}.
   Context `{Hdr_finite: @Finite Hdr _ Hdr_eq_dec}.
-  Variable (sz: Hdr -> nat).
+  Variable (Hdr_sz: Hdr -> nat).
 
-  Variable (a: P4A.t St sz).
+  Variable (a: P4A.t St Hdr_sz).
 
   Equations compile_store_ctx_partial
     (hdrs: list Hdr)
@@ -38,7 +38,7 @@ Section CompileFirstOrderConfRelSimplified.
   := {
     compile_store_ctx_partial nil := CEmp _;
     compile_store_ctx_partial (hdr :: hdrs) :=
-      CSnoc _ (compile_store_ctx_partial hdrs) (FOBV.Bits (sz hdr))
+      CSnoc _ (compile_store_ctx_partial hdrs) (FOBV.Bits (Hdr_sz hdr))
   }.
 
   Definition compile_store_ctx : ctx FOBV.sig :=
@@ -46,7 +46,7 @@ Section CompileFirstOrderConfRelSimplified.
 
   Equations compile_store_valu_partial
     {hdrs: list Hdr}
-    (hl: HList.t (fun h => (n_tuple bool (sz h))) hdrs)
+    (hl: HList.t (fun h => (n_tuple bool (Hdr_sz h))) hdrs)
     : valu FOBV.sig FOBV.fm_model (compile_store_ctx_partial hdrs)
       by struct hl
   := {
@@ -56,7 +56,7 @@ Section CompileFirstOrderConfRelSimplified.
             (compile_store_valu_partial hdrs)
   }.
 
-  Equations compile_ctx (c: ctx (FOS.sig sz)) : ctx FOBV.sig := {
+  Equations compile_ctx (c: ctx (FOS.sig Hdr_sz)) : ctx FOBV.sig := {
     compile_ctx (CEmp _) := CEmp _;
     compile_ctx (CSnoc _ c FOS.Store) :=
       app_ctx (compile_ctx c) compile_store_ctx;
@@ -66,19 +66,19 @@ Section CompileFirstOrderConfRelSimplified.
 
   Equations build_hlist_env
     (hdrs: list Hdr)
-    (env: P4A.store Hdr sz)
-    : (HList.t (fun h => (n_tuple bool (sz h))) hdrs) := {
+    (env: P4A.store Hdr Hdr_sz)
+    : (HList.t (fun h => (n_tuple bool (Hdr_sz h))) hdrs) := {
       build_hlist_env nil _ := hnil;
       build_hlist_env (hdr :: hdrs) env :=
-        let v := match P4A.find Hdr sz hdr env with
+        let v := match P4A.find Hdr Hdr_sz hdr env with
                  | P4A.VBits _ v => v
                  end in
         (_ v) ::: build_hlist_env hdrs env
     }.
 
   Equations compile_valu
-    {c: ctx (FOS.sig sz)}
-    (v: valu (FOS.sig sz) (FOS.fm_model a) c)
+    {c: ctx (FOS.sig Hdr_sz)}
+    (v: valu (FOS.sig Hdr_sz) (FOS.fm_model a) c)
     : valu FOBV.sig FOBV.fm_model (compile_ctx c) := {
     compile_valu (VEmp _ _) := VEmp _ _;
     compile_valu (VSnoc _ _ (FOS.Bits n) _ v vinner) :=
@@ -110,24 +110,24 @@ Section CompileFirstOrderConfRelSimplified.
     (enum: list Hdr)
     (elem_of_enum: List.In k enum)
     : var (FOBV.sig) (compile_store_ctx_partial enum)
-          (FOBV.Bits (sz k)) := {
+          (FOBV.Bits (Hdr_sz k)) := {
     compile_lookup_partial k (elem :: enum) elem_of_enum :=
       match here_or_there elem_of_enum with
       | left Heq =>
-        _ (VHere _ (compile_store_ctx_partial enum) (FOBV.Bits (sz elem)))
+        _ (VHere _ (compile_store_ctx_partial enum) (FOBV.Bits (Hdr_sz elem)))
       | right Helse =>
-        VThere FOBV.sig _ (FOBV.Bits (sz elem))
+        VThere FOBV.sig _ (FOBV.Bits (Hdr_sz elem))
                _ (compile_lookup_partial k enum Helse)
       end
   }.
 
   Definition compile_lookup (k: Hdr)
-    : var FOBV.sig compile_store_ctx (FOBV.Bits (sz k))
+    : var FOBV.sig compile_store_ctx (FOBV.Bits (Hdr_sz k))
   :=
     compile_lookup_partial k (enum Hdr) (elem_of_enum k).
 
   Definition get_sizes (enum: list Hdr) : list nat :=
-    List.map sz enum.
+    List.map Hdr_sz enum.
 
   Definition compile_sizes (enum: list Hdr) : nat :=
     List.list_sum (get_sizes enum).
@@ -144,7 +144,7 @@ Section CompileFirstOrderConfRelSimplified.
                   (FOBV.Bits (compile_sizes enum)) := {
     compile_store_partial nil := TFun FOBV.sig (FOBV.BitsLit 0 tt) hnil;
     compile_store_partial (elem :: enum) :=
-      TFun FOBV.sig (FOBV.Concat (sz elem) (compile_sizes enum))
+      TFun FOBV.sig (FOBV.Concat (Hdr_sz elem) (compile_sizes enum))
                     (TVar (VHere _ _ _) :::
                      tm_cons FOBV.sig (compile_store_partial enum) ::: hnil)
   }.
@@ -155,7 +155,7 @@ Section CompileFirstOrderConfRelSimplified.
     compile_store_partial (enum Hdr).
 
   Equations subscript {c n}
-    (v: var (FOS.sig sz) c FOS.Store)
+    (v: var (FOS.sig Hdr_sz) c FOS.Store)
     (v': var FOBV.sig compile_store_ctx (FOBV.Bits n))
     : var FOBV.sig (compile_ctx c) (FOBV.Bits n)
   := {
@@ -168,9 +168,9 @@ Section CompileFirstOrderConfRelSimplified.
   }.
 
   Equations compile_var
-    {c: ctx (FOS.sig sz)}
+    {c: ctx (FOS.sig Hdr_sz)}
     {s: FOS.sorts}
-    (v: var (FOS.sig sz) c s)
+    (v: var (FOS.sig Hdr_sz) c s)
     : tm FOBV.sig (compile_ctx c) (compile_sort s)
   := {
     compile_var (VHere _ c (FOS.Bits n)) :=
@@ -181,9 +181,9 @@ Section CompileFirstOrderConfRelSimplified.
   }.
 
   Equations compile_tm
-    {c: ctx (FOS.sig sz)}
+    {c: ctx (FOS.sig Hdr_sz)}
     {s: FOS.sorts}
-    (t: tm (FOS.sig sz) c s):
+    (t: tm (FOS.sig Hdr_sz) c s):
     tm FOBV.sig (compile_ctx c) (compile_sort s) := {
     compile_tm (TVar v) := compile_var v;
     compile_tm (TFun _ (FOS.BitsLit _ n v) hnil) :=
@@ -198,8 +198,8 @@ Section CompileFirstOrderConfRelSimplified.
   }.
 
   Equations compile_fm
-    {c: ctx (FOS.sig sz)}
-    (f: fm (FOS.sig sz) c)
+    {c: ctx (FOS.sig Hdr_sz)}
+    (f: fm (FOS.sig Hdr_sz) c)
     : fm FOBV.sig (compile_ctx c) := {
     compile_fm FTrue := FTrue;
     compile_fm FFalse := FFalse;
@@ -221,7 +221,7 @@ Section CompileFirstOrderConfRelSimplified.
   := {
     compile_store_val_partial s nil := tt;
     compile_store_val_partial s (elem :: enum) :=
-      let '(P4A.VBits _ v) := P4A.find Hdr sz elem s in
+      let '(P4A.VBits _ v) := P4A.find Hdr Hdr_sz elem s in
       n_tuple_concat v (compile_store_val_partial s enum)
   }.
 
@@ -239,9 +239,9 @@ Section CompileFirstOrderConfRelSimplified.
 
   Lemma compile_store_val_correct':
     forall (h : Hdr)
-      (m : mod_sorts (FOS.sig sz) (FOS.fm_model a) FOS.Store) enum Hin,
+      (m : mod_sorts (FOS.sig Hdr_sz) (FOS.fm_model a) FOS.Store) enum Hin,
     List.NoDup enum ->
-    match P4A.find Hdr sz h m with
+    match P4A.find Hdr Hdr_sz h m with
     | P4A.VBits _ v1 => v1
     end =
     find FOBV.sig FOBV.fm_model
@@ -266,13 +266,13 @@ Section CompileFirstOrderConfRelSimplified.
         unfold equiv in e.
         dependent destruction e.
         cbn.
-        now rewrite (find_equation_1 FOBV.sig FOBV.fm_model (compile_store_ctx_partial enum) (FOBV.Bits (sz h))).
+        now rewrite (find_equation_1 FOBV.sig FOBV.fm_model (compile_store_ctx_partial enum) (FOBV.Bits (Hdr_sz h))).
       + unfold here_or_there.
         destruct (equiv_dec _ _); simpl.
         unfold equiv in e.
         inversion H.
         congruence.
-        rewrite (find_equation_2 FOBV.sig FOBV.fm_model (compile_store_ctx_partial enum) (FOBV.Bits (sz a0)) (FOBV.Bits (sz h))).
+        rewrite (find_equation_2 FOBV.sig FOBV.fm_model (compile_store_ctx_partial enum) (FOBV.Bits (Hdr_sz a0)) (FOBV.Bits (Hdr_sz h))).
         apply IHenum.
         now inversion H.
   Qed.
@@ -280,8 +280,8 @@ Section CompileFirstOrderConfRelSimplified.
   Opaque compile_store_valu_partial.
 
   Lemma compile_store_val_correct:
-    forall (h : Hdr) c (v0 : var (FOS.sig sz) c FOS.Store) v,
-      match P4A.find Hdr sz h (find (FOS.sig sz) (FOS.fm_model a) v0 v)
+    forall (h : Hdr) c (v0 : var (FOS.sig Hdr_sz) c FOS.Store) v,
+      match P4A.find Hdr Hdr_sz h (find (FOS.sig Hdr_sz) (FOS.fm_model a) v0 v)
       with
       | P4A.VBits _ v1 => v1
       end =
@@ -306,7 +306,7 @@ Section CompileFirstOrderConfRelSimplified.
       + simpl.
         rewrite (subscript_equation_2 n (ctx1 := c) v0 (compile_lookup h)).
         rewrite (compile_valu_equation_2 n (c0 := c) m).
-        now rewrite (find_equation_2 FOBV.sig FOBV.fm_model (compile_ctx c) (FOBV.Bits n) (FOBV.Bits (sz h))).
+        now rewrite (find_equation_2 FOBV.sig FOBV.fm_model (compile_ctx c) (FOBV.Bits n) (FOBV.Bits (Hdr_sz h))).
       + rewrite (subscript_equation_3 (ctx1 := c) v0).
         rewrite (compile_valu_equation_3 (c0 := c) m v).
         erewrite <- find_app_left; now f_equal.
@@ -315,32 +315,32 @@ Section CompileFirstOrderConfRelSimplified.
   Equations decompile_store_val_partial
     (enum: list Hdr)
     (val: n_tuple bool (compile_sizes enum))
-    (store: P4A.store Hdr sz)
-    : P4A.store Hdr sz
+    (store: P4A.store Hdr Hdr_sz)
+    : P4A.store Hdr Hdr_sz
   := {
     decompile_store_val_partial nil val store := store;
     decompile_store_val_partial (elem :: enum) val store :=
-      let prefix := rewrite_size _ (n_tuple_take_n (sz elem) val) in
-      let suffix := rewrite_size _ (n_tuple_skip_n (sz elem) val) in
-      P4A.assign Hdr sz elem (P4A.VBits _ prefix)
+      let prefix := rewrite_size _ (n_tuple_take_n (Hdr_sz elem) val) in
+      let suffix := rewrite_size _ (n_tuple_skip_n (Hdr_sz elem) val) in
+      P4A.assign Hdr Hdr_sz elem (P4A.VBits _ prefix)
                  (decompile_store_val_partial enum suffix store)
   }.
   Next Obligation.
     unfold compile_sizes.
     simpl.
     remember (List.list_sum _).
-    remember (sz elem).
+    remember (Hdr_sz elem).
     Lia.lia.
   Defined.
   Next Obligation.
     unfold compile_sizes.
     simpl.
     remember (List.list_sum _).
-    remember (sz elem).
+    remember (Hdr_sz elem).
     Lia.lia.
   Defined.
 
-  Definition init_store: P4A.store Hdr sz.
+  Definition init_store: P4A.store Hdr Hdr_sz.
   Proof.
     apply DepEnv.init.
     intro.
@@ -362,7 +362,7 @@ Section CompileFirstOrderConfRelSimplified.
   Lemma compile_store_val_partial_invariant:
     forall h v enum s,
       ~ List.In h enum ->
-      compile_store_val_partial (P4A.assign Hdr sz h v s) enum =
+      compile_store_val_partial (P4A.assign Hdr Hdr_sz h v s) enum =
       compile_store_val_partial s enum.
   Proof.
     intros.
@@ -391,7 +391,7 @@ Section CompileFirstOrderConfRelSimplified.
       simpl.
       rewrite P4A.assign_find; auto.
       symmetry.
-      rewrite <- NtupleProofs.n_tuple_concat_roundtrip with (n := sz a0).
+      rewrite <- NtupleProofs.n_tuple_concat_roundtrip with (n := Hdr_sz a0).
       symmetry.
       apply NtupleProofs.concat_proper with
         (xs2 := (rewrite_size (decompile_store_val_partial_obligations_obligation_1 a0 enum) _))
@@ -417,7 +417,7 @@ Section CompileFirstOrderConfRelSimplified.
   Qed.
 
   Definition store_almost_equal (s1 s2: store (P4A.interp a)) :=
-    forall (h: Hdr), P4A.find Hdr sz h s1 = P4A.find Hdr sz h s2.
+    forall (h: Hdr), P4A.find Hdr Hdr_sz h s1 = P4A.find Hdr Hdr_sz h s2.
 
   Theorem store_eq:
     forall (s1 s2: store (P4A.interp a)),
@@ -454,12 +454,12 @@ Section CompileFirstOrderConfRelSimplified.
           simpl.
           rewrite P4A.assign_find;
             try solve [eauto | typeclasses eauto].
-          destruct (P4A.find Hdr sz a0 val).
+          destruct (P4A.find Hdr Hdr_sz a0 val).
           f_equal.
           apply JMeq_eq.
           rewrite rewrite_size_jmeq.
           pose proof NtupleProofs.n_tuple_take_n_roundtrip.
-          now specialize (H0 (sz a0) n _ (compile_store_val_partial val l)).
+          now specialize (H0 (Hdr_sz a0) n _ (compile_store_val_partial val l)).
         * unfold equiv, complement in c.
           autorewrite with compile_store_val_partial.
           autorewrite with decompile_store_val_partial.
@@ -467,11 +467,11 @@ Section CompileFirstOrderConfRelSimplified.
           rewrite P4A.find_not_first by assumption.
           rewrite IHl by (destruct H; congruence).
           do 2 f_equal.
-          destruct (P4A.find Hdr sz a0 val).
+          destruct (P4A.find Hdr Hdr_sz a0 val).
           apply JMeq_eq.
           rewrite rewrite_size_jmeq.
           pose proof NtupleProofs.n_tuple_skip_n_roundtrip.
-          now specialize (H0 (sz a0) n _ (compile_store_val_partial val l)).
+          now specialize (H0 (Hdr_sz a0) n _ (compile_store_val_partial val l)).
   Qed.
 
   Lemma compile_store_val_partial_correct':
@@ -487,7 +487,7 @@ Section CompileFirstOrderConfRelSimplified.
       autorewrite with build_hlist_env.
       simpl.
       unfold build_hlist_env_obligations_obligation_1.
-      destruct (P4A.find Hdr sz a0 m).
+      destruct (P4A.find Hdr Hdr_sz a0 m).
       rewrite (compile_store_valu_partial_equation_2 a0 (rest := enum) n).
       rewrite (compile_store_partial_equation_2 a0 enum).
       autorewrite with interp_tm; simpl.
@@ -587,7 +587,7 @@ Section CompileFirstOrderConfRelSimplified.
   Lemma compile_store_valu_partial_invariant:
     forall h v enum s,
       ~ List.In h enum ->
-      compile_store_valu_partial (build_hlist_env enum (P4A.assign Hdr sz h v s)) =
+      compile_store_valu_partial (build_hlist_env enum (P4A.assign Hdr Hdr_sz h v s)) =
       compile_store_valu_partial (build_hlist_env enum s).
   Proof.
     induction enum; intros.
@@ -597,7 +597,7 @@ Section CompileFirstOrderConfRelSimplified.
       unfold build_hlist_env_obligations_obligation_1.
       rewrite P4A.find_not_first;
         try solve [typeclasses eauto | eauto].
-      + destruct (P4A.find Hdr sz a0 s).
+      + destruct (P4A.find Hdr Hdr_sz a0 s).
         specialize (IHenum s).
         rewrite (compile_store_valu_partial_equation_2 _ (rest := enum)).
         rewrite (compile_store_valu_partial_equation_2 _ (rest := enum)).
@@ -614,7 +614,7 @@ Section CompileFirstOrderConfRelSimplified.
     forall enum,
       List.NoDup enum ->
       forall (val: valu FOBV.sig FOBV.fm_model (compile_store_ctx_partial enum)),
-        exists s: P4A.store Hdr sz,
+        exists s: P4A.store Hdr Hdr_sz,
           compile_store_valu_partial (build_hlist_env enum s) = val.
   Proof.
     induction enum; intros.
@@ -626,7 +626,7 @@ Section CompileFirstOrderConfRelSimplified.
       inversion H.
       specialize (IHenum H3 val).
       destruct IHenum as [? ?].
-      exists (P4A.assign Hdr sz a0 (P4A.VBits _ m) x0).
+      exists (P4A.assign Hdr Hdr_sz a0 (P4A.VBits _ m) x0).
       autorewrite with build_hlist_env.
       simpl.
       unfold build_hlist_env_obligations_obligation_1.
@@ -639,7 +639,7 @@ Section CompileFirstOrderConfRelSimplified.
 
   Lemma compile_store_valu_partial_surjective:
     forall (val: valu FOBV.sig FOBV.fm_model compile_store_ctx),
-      exists s: P4A.store Hdr sz,
+      exists s: P4A.store Hdr Hdr_sz,
         compile_store_valu_partial (build_hlist_env (enum Hdr) s) = val.
   Proof.
     intros.
